src/Repr/SystemFOp/Type.v
@@ -2,10 +2,7 @@ Require Import List.
 
 Require Import Repr.Lists.
 
-Require Import Repr.Tactics.All.
-Require Import Repr.Tactics.Rewrite.
-Require Import Repr.Tactics.Burn.
-Require Import Repr.Tactics.Norm.
+Require Import Repr.Tactics.
 Require Import Repr.Tactics.LibTactics.
 
 Require Import Coq.Arith.Peano_dec.
@@ -50,11 +47,15 @@ Hint Constructors well_formed_typ.
 (* A type is closed if it is well-formed in the empty kind environment *)
 Definition closed_typ (T:typ) : Prop := well_formed_typ nil T.
 
+(* Trick to control how far simpl goes for better automation *)
+Definition lift_le_gt_dec (n m : nat) := le_gt_dec n m.
+Arguments lift_le_gt_dec _ _ : simpl nomatch.
+
 (* Standard de bruijn lifting and substituion functions operating at the type level *)
 Fixpoint typ_lift (dp:nat)(T:typ) : typ :=
   match T with
     | TVar X =>
-       if (le_gt_dec dp X) then TVar (S X) else TVar X
+       if (lift_le_gt_dec dp X) then TVar (S X) else TVar X
     | TNat => 
        TNat
     | TArrow T1 T2 =>
@@ -126,6 +127,111 @@ Ltac inverts_typ :=
 Tactic Notation "induction_kind" ident(t) :=
   induction t; rip; simpl; inverts_typ; tburn.
 
+
+(********************************************************************)
+(* Lemmas for manipulating the lifting and substitution operations. *)
+
+(* Handy tactic for burning down TVar case analysis which usually boils down
+ * to repeated less than and nat compares *)
+
+Ltac case_lift :=
+  match goal with
+    | [ |- context [lift_le_gt_dec ?a ?b] ] =>
+      case (lift_le_gt_dec a b)
+  end.
+
+Ltac burn_tvar :=
+  simpl;
+  match goal with
+    | [ |- context[nat_compare _ _ ] ]
+      => break_nat_compare ;
+         tburn;
+         burn_tvar
+    | [ |- context [lift_le_gt_dec _ _ ] ]
+      => case_lift ;
+         tburn;
+         burn_tvar
+    | _ 
+      => tburn
+  end.
+
+Lemma typ_subs_nil_typ_lift
+  :  forall X U T
+  ,  [X |=> U] (typ_lift X T) = T.
+Proof.
+  rip; gen X U; induction_kind T; destruct X; burn_tvar.
+Qed.
+Hint Rewrite typ_subs_nil_typ_lift.
+
+Lemma tall_injective 
+  :  forall (T1 T2:typ)
+  ,  T1 = T2
+  -> TAll T1 = TAll T2.
+Proof. burn. Qed.
+
+Lemma typ_lift_SX
+  :  forall (X Y:tvar)(T:typ)
+  ,  Y <= X
+  -> typ_lift (S X) (typ_lift Y T) = typ_lift Y (typ_lift X T).
+Proof.
+  rip; gen X Y; induction T; tburn; rip; burn_tvar.
+Qed.  
+
+Lemma typ_lift_over_subs
+  :  forall (n n':nat)(U T:typ)
+  ,  typ_lift n ([(n + n') |=> U] T) 
+  =  [(1 + n + n') |=> typ_lift n U] typ_lift n T.
+Proof.
+  rip; gen n n' U; induction T; tburn.
+  rip; burn_tvar.
+
+  rip; simpl; eapply tall_injective.
+  assert (S (n + n') = S n + n'). burn. rewrite H. rewrite IHT. simpl.
+
+  rewrite typ_lift_SX; burn. 
+Qed.
+Hint Rewrite typ_lift_over_subs.
+
+Lemma typ_lift_over_subs'
+  :  forall (n n':nat)(U T:typ)
+  ,  typ_lift (n + n') ([n |=> U] T) 
+  =  [n  |=> typ_lift (n + n') U] typ_lift (1 + n + n') T.
+Proof.
+  rip; gen n n' U; induction T; tburn.
+  
+  rip; destruct n; burn_tvar.
+
+  rip. simpl. eapply tall_injective. 
+  assert (S (n + n') = S n + n'). burn. rewrite H. rewrite IHT. simpl.
+  rewrite typ_lift_SX; burn.
+Qed.
+Hint Rewrite typ_lift_over_subs.
+
+(* LAST : Solve *)
+
+Lemma commute_typ_subs
+  :  forall (n n':nat)(T1 T2 T3:typ)
+  ,  [n + n' |=> T3] ([n |=> T2] T1)
+  =  [n |=> [ n + n' |=> T3] T2 ] ([1 + n + n' |=> (typ_lift n T3)] T1).
+Proof.
+  rip; gen n n' T2 T3 ; induction_kind T1.
+  burn_tvar.
+  break (nat_compare n (S (n + n'))); norm_nat_compare; simpl; tburn.
+  burn_tvar.
+  
+  eapply tall_injective.
+  assert (n + n' = 0 + (n + n')) by burn. rewrite H at 2.
+  rewrite typ_lift_over_subs; simpl.
+  
+  assert (S (n + n') = S n + n') by burn. rewrite H0.
+  assert (S (S n + n') = 1 + S n + n') by burn. rewrite H1.
+  rewrite IHT1.
+  rewrite typ_lift_SX; burn.
+Qed.
+
+
+(********************************************************************)
+
 (* A well-kinded type is well-formed *)
 Lemma kind_rel_imp_well_formed_typ
   :  forall D T K
@@ -134,6 +240,7 @@ Lemma kind_rel_imp_well_formed_typ
 Proof.
   rip; gen D K; induction_kind T.
 Qed.
+Hint Resolve kind_rel_imp_well_formed_typ.
 
 (* We may insert into a kind environment at X provided we lift all
  * types that occuring after X in the kind environment. 
@@ -153,8 +260,8 @@ Proof.
   rip; gen D K X; induction_kind T;
   match goal with
     (* TVar *)
-    | [ |- context [le_gt_dec ?A ?B] ] 
-      => break (le_gt_dec A B); tburn
+    | [ |- context [lift_le_gt_dec ?A ?B] ] 
+      => break (lift_le_gt_dec A B); tburn
     (* TAbs *)
     | _ 
       => econstructor; autorewrite_goal; burn
@@ -163,106 +270,34 @@ Proof.
 Qed.
 Hint Resolve kind_rel_insert.
 
-Lemma cons_eq_insert0
-  :  forall X (ls: list X)(e:X)
-  ,  e :: ls = insert ls 0 e.
-Proof.
-  destruct ls; burn.
-Qed.  
-
 Theorem kind_rel_weakening
   :  forall D T K
   ,  D \\- T \: K
   -> (KStar :: D) \\- typ_lift 0 T \: K.
 Proof.
-  rip; rewrite cons_eq_insert0; burn.
+  rip; rewrite cons_as_insert; burn.
 Qed.  
+Hint Resolve kind_rel_weakening.
 
-(********************************************************************)
-(* Lemmas for manipulating the lifting and substitution operations. *)
-
-(* Handy tactic for burning down TVar case analysis which usually boils down
- * to repeated less than and nat compares *)
-Ltac burn_tvar :=
-  repeat(
-    simpl;
-    try break_nat_compare;
-    tburn;
-    match goal with
-      | [ |- context[le_gt_dec ?X ?Y] ] => break (le_gt_dec X Y)
-    end;
-    tburn
-  ).
-
-Ltac case_lift :=
-  match goal with
-    | [ |- context [le_gt_dec ?a ?b] ] =>
-      case (le_gt_dec a b)
-  end.
-
-Lemma typ_subs_nil_typ_lift
-  :  forall X U T
-  ,  [X |=> U] (typ_lift X T) = T.
+Lemma type_substition_preserves_kinding'
+  :  forall (D:kenv)(X:tvar)(U T:typ)
+  ,  delete D X \\- U \: KStar
+  -> D \\- T \: KStar
+  -> delete D X \\- [X |=> U] T \: KStar.
 Proof.
-  rip; gen X U; induction_kind T; destruct X;
-  case_lift; burn_tvar. 
+  rip; gen D X U; induction_kind T.
+  burn_tvar. econstructor. burn.
+  econstructor; rewrite delete_rewind; eapply IHT; burn.
 Qed.
-Hint Rewrite typ_subs_nil_typ_lift.
+Hint Resolve type_substition_preserves_kinding'.
 
-Lemma tall_injective 
-  :  forall (T1 T2:typ)
-  ,  T1 = T2
-  -> TAll T1 = TAll T2.
-Proof. burn. Qed.
+Lemma type_substition_preserves_kinding
+  :  forall (D:kenv)(X:tvar)(U T:typ)
+  ,  delete (KStar :: D) 0 \\- U \: KStar
+  -> (KStar :: D) \\- T \: KStar
+  -> delete (KStar :: D) 0 \\- [0 |=> U] T \: KStar.
+Proof. rip; burn. Qed.
 
-Lemma typ_lift_SX
-  :  forall (X Y:tvar)(T:typ)
-  ,  Y <= X
-  -> typ_lift Y (typ_lift X T) = typ_lift (S X) (typ_lift Y T).
-Proof.
-  rip; gen X Y; induction T; tburn.
-
-  rip;
-  rename t into Z;
-  break Z;
-  repeat(
-    simpl;
-    match goal with 
-      | [ |- context[le_gt_dec ?X ?Y] ] =>
-        break (le_gt_dec X Y)
-    end;
-    tburn
-  ).
-Qed.  
-
-Lemma typ_lift_over_subs
-  :  forall (n n':nat)(U T:typ)
-  ,  typ_lift n ([(n + n') |=> U] T) 
-  =  [(1 + n + n') |=> typ_lift n U] typ_lift n T.
-Proof.
-  rip; gen n n' U; induction T; tburn.
-  rip; burn_tvar.
-
-  rip; simpl; eapply tall_injective.
-  assert (S (n + n') = S n + n'). burn. rewrite H. rewrite IHT. simpl.
-  
-
-  rewrite <- typ_lift_SX; burn. 
-Qed.
-Hint Rewrite typ_lift_over_subs.
-
-(* LAST *)
-
-Lemma typ_lift_over_subs'
-  :  forall (n n':nat)(U T:typ)
-  ,  typ_lift (n + n') ([n |=> U] T) 
-  =  [n  |=> typ_lift (n + n') U] typ_lift (1 + n + n') T.
-Proof.
-  rip; gen n n' U; induction T; tburn.
-
-
-Qed.
-Hint Rewrite typ_lift_over_subs.
 
 (********************************************************************)
 
@@ -280,5 +315,74 @@ Definition tenv_substitute (X:tvar)(U:typ)(G:tenv) : tenv :=
   map (typ_substitute X U) G.
 Hint Unfold tenv_substitute.
 
+(********************************************************************)
 
+Lemma delete_tenv_lift 
+  :  forall G x
+  ,  delete (tenv_lift 0 G) x = tenv_lift 0 (delete G x).
+Proof.
+  rip; gen G; induction x; destruct G; tburn.
+Qed.
+
+Lemma get_tenv_lift
+  :  forall G x T X
+  ,  get G x = Some T
+  -> get (tenv_lift X G) x = Some (typ_lift X T).
+Proof.
+  induction G; destruct x; rip; 
+  simpl in *; try norm_some; tburn.
+Qed.
+Hint Resolve get_tenv_lift.
+
+Lemma rewind_tenv_lift
+  :  forall G T X
+  ,  typ_lift X T :: tenv_lift X G = tenv_lift X (T :: G).
+Proof. burn. Qed.
+Hint Rewrite rewind_tenv_lift.
+
+Lemma tenv_lift_SX
+  :  forall G X
+  ,  tenv_lift 0 (tenv_lift X G) = tenv_lift (S X) (tenv_lift 0 G).
+Proof.
+  induction G; rip; simpl; tburn.
+  rewrite IHG; rewrite typ_lift_SX; burn.
+Qed.
+
+Lemma get_tenv_substitute
+  :  forall G X Y U T
+  ,  get G Y = Some T
+  -> get (tenv_substitute X U G) Y = Some ([X |=> U] T).
+Proof.  
+  induction G; destruct Y; rip;
+  simpl in *; try norm_some; tburn.
+Qed.
+Hint Resolve get_tenv_substitute.
+
+Lemma rewind_tenv_substitute
+  :  forall G U T X
+  ,  [X |=> U] T :: tenv_substitute X U G = tenv_substitute X U (T :: G).
+Proof. burn. Qed.
+Hint Rewrite rewind_tenv_substitute.
+
+Lemma typ_lift_over_tenv_subs
+  :  forall (n n':nat)(U:typ)(D:tenv)
+  ,  tenv_lift n (tenv_substitute (n + n') U D) 
+  =  tenv_substitute (1 + n + n') (typ_lift n U) (tenv_lift n D).
+Proof.
+  rip; gen n n' U; induction D; tburn.
+  rip. simpl. rewrite IHD. simpl.
+  burn.
+Qed.
+Hint Rewrite typ_lift_over_tenv_subs.
+
+Lemma typ_lift_over_tenv_subs'
+  :  forall (n n':nat)(U:typ)(D:tenv)
+  ,  tenv_lift (n + n') (tenv_substitute n U D) 
+  =  tenv_substitute n (typ_lift (n + n') U) (tenv_lift (1 + n + n') D).
+Proof.
+  rip; gen n n' U; induction D; tburn.
+  rip. simpl. rewrite IHD. simpl. 
+  rewrite typ_lift_over_subs'. burn.
+Qed.
+Hint Rewrite typ_lift_over_tenv_subs'.
 
