src/Repr/SystemFOp/TypeRel.v
@@ -51,10 +51,10 @@ Inductive type_rel : kenv -> tenv -> term -> typ -> Prop :=
         (KStar :: D), (tenv_lift 0 G) ||- t \: T ->
         D, G ||- (TyAbs t) \: TAll T
   | TR_TyApp :
-      forall D G t T ty, 
+      forall D G t T T', 
         D, G ||- t \: TAll T ->
-        D \\- ty \: KStar ->
-        D, G ||- (TyApp t ty) \: [0 |=> ty] T
+        D \\- T' \: KStar ->
+        D, G ||- (TyApp t T') \: [0 |=> T'] T
 
 where "D ',' G '||-' t '\:' T" := (type_rel D G t T).
 
@@ -82,29 +82,14 @@ Ltac inverts_term :=
 Tactic Notation "induction_type" ident(t) :=
   induction t; rip; simpl; inverts_term; tburn.
 
-Lemma get_lift
-  :  forall (G:tenv)(x:var)(T:typ)(X:tvar)
-  ,  get G x = Some T
-  -> get (tenv_lift X G) x = Some (typ_lift X T).
+Lemma type_rel_imp_wellformed_term
+  :  forall (D:kenv)(G:tenv)(t:term)(T:typ)
+  ,  D, G ||- t \: T
+  -> well_formed_term D G t.
 Proof.
-  induction G; destruct x; rip; 
-  simpl in *; try norm_some; tburn.
+  rip; gen D G T; induction_type t.
 Qed.
-Hint Resolve get_lift.
-
-Lemma rewind_typ_lift
-  :  forall (G:tenv)(T:typ)(X:tvar)
-  ,  typ_lift X T :: tenv_lift X G = tenv_lift X (T :: G).
-Proof. tburn. Qed.
-Hint Rewrite rewind_typ_lift.
-
-Lemma tenv_lift_SX
-  :  forall (G:tenv)(X:tvar)
-  ,  tenv_lift 0 (tenv_lift X G) = tenv_lift (S X) (tenv_lift 0 G).
-Proof.
-  induction G; rip; simpl; tburn.
-  rewrite IHG; rewrite typ_lift_SX; burn.
-Qed.
+Hint Resolve type_rel_imp_wellformed_term.
 
 (* Lemma used to prove kenv_weaking (since its induction hypothesis is not
    strong enough.
@@ -117,7 +102,7 @@ Lemma kenv_insert
   -> (insert D X KStar), (tenv_lift X G) ||- (typ_term_lift X t) \: (typ_lift X T).
 Proof.
   rip; gen D G T X; induction_type t.
-
+ 
   (* Add *)
   assert (TNat = typ_lift X TNat).
     burn.
@@ -131,57 +116,209 @@ Proof.
   burn.
 
   (* TyApp *)
+  break (nat_compare X 0); norm_nat_compare.
   
-  
-  
-  
-  
-  
-  
+    (* Case X = 0 *)
+    subst.
+    assert (0 = 0+0). burn. rewrite H at 5.
+    rewrite typ_lift_over_subs'. simpl. 
+    econstructor; burn.
 
+    (* Case X < 0 *)
+    burn.
+
+    (* Case X > 0 *)
+    assert (X = 0+X). burn. rewrite H at 5.
+    rewrite typ_lift_over_subs'. simpl.
+    econstructor; burn.
 Qed.  
+
+Lemma kenv_weakening
+  :  forall (D:kenv)(G:tenv)(t:term)(T:typ)(X:tvar)
+  ,  D, G ||- t \: T
+  -> (KStar :: D), (tenv_lift 0 G) ||- (typ_term_lift 0 t) \: (typ_lift 0 T).
+Proof.
+  rip; rewrite cons_as_insert; apply kenv_insert; burn.
+Qed.
+Hint Resolve kenv_weakening.
 
 Lemma tenv_weakening
   :  forall (D:kenv)(G:tenv)(t:term)(T:typ)(x:var)
   ,  D, delete G x ||- t \: T
   -> D, G ||- term_lift x t \: T.
 Proof.
-  rip; gen G T x; induction_type t.
+  rip; gen D G T x; induction_type t.
   match goal with
-    | [ |- context[le_gt_dec ?X ?Y] ] 
-      => break (le_gt_dec X Y); tburn;
+    | [ |- context[lift_le_gt_dec ?X ?Y] ] 
+      => break (lift_le_gt_dec X Y); tburn;
          constructor; rewrite get_delete_above_idx in *; tburn
   end.
-Qed.
-Hint Resolve env_weakening.
 
-Lemma tm_substition_preserves_typing' 
-  :  forall (G:env)(x:var)(s t:term)(U T:typ)
-  ,  get G x = Some (term,U) 
-  -> delete G x ||- s \: U 
-  -> G ||- t \: T 
-  -> delete G x ||- [x ~> s] t \: T.
+  econstructor. eapply IHt. rewrite delete_tenv_lift. burn.
+Qed.
+Hint Resolve tenv_weakening.
+
+Lemma type_substition_preserves_typing'
+  :  forall (D:kenv)(G:tenv)(X:tvar)(t:term)(U T:typ)
+  ,  delete D X \\- U \: KStar
+  -> D, G ||- t \: T
+  -> delete D X, (tenv_substitute X U G) ||- [X ~~> U] t \: [X |=> U] T.
 Proof.
-  rip; gen G x s U T; induction_type t;
+  rip; gen D G X U T; induction_type t.
+
+  (* TR-Nat *)
+  assert (TNat = [X |=> U] TNat). burn.
+  econstructor. burn. burn.
+
+  (* TR-Abs *)
+  simpl. econstructor. eapply type_substition_preserves_kinding'; burn.
+  rewrite rewind_tenv_substitute. burn.
+
+  (* TR-App *)
+  econstructor. specialize (IHt1 _ _ _ _ H _ H5). simpl in IHt1. eassumption.
+  eapply IHt2; burn.
+
+  (* TR-TyAbs *)
+  simpl. econstructor.
+  assert (X = 0 + X) by burn. rewrite H0 at 2; clear H0.
+  rewrite typ_lift_over_tenv_subs; simpl.
+  rewrite delete_rewind. 
+  eapply IHt; tburn.
+
+  (* TR-TyApp *)
+  rename t0 into T'. rewrite (commute_typ_subs 0 X); simpl; tburn.
+  eapply TR_TyApp; tburn.
+  assert (TAll ([S X |=> typ_lift 0 U] T0) = [X |=> U] TAll T0) by burn.
+  rewrite H0; burn.
+Qed.
+
+Lemma type_substition_preserves_typing
+  :  forall (D:kenv)(G:tenv)(t:term)(U T:typ)
+  ,  D \\- U \: KStar
+  ->  (KStar :: D), G ||- t \: T 
+  -> D, (tenv_substitute 0 U G) ||- [0 ~~> U] t \: [0 |=> U] T.
+Proof.
+  rip; eapply (type_substition_preserves_typing' (KStar :: D) _ 0); burn.
+Qed.
+Hint Resolve type_substition_preserves_typing.
+
+Lemma term_substition_preserves_typing' 
+  :  forall (D:kenv)(G:tenv)(x:var)(s t:term)(U T:typ)
+  ,  get G x = Some U 
+  -> D, delete G x ||- s \: U 
+  -> D, G ||- t \: T 
+  -> D, delete G x ||- [x ~> s] t \: T.
+Proof.
+  rip; gen D G x s U T; induction_type t;
   match goal with
     (* TVar *)
     | [ |- context [ nat_compare _ _ ] ] 
       => break_nat_compare; tburn; constructor; tburn
     (* TAbs *)                                              
-    | [ |- context [ Abs _ ]           ]
-      => econstructor; rewrite delete_rewind; tburn
-  end.
+    | [ |- context [ Abs _ _ ]         ]
+      => econstructor; try rewrite delete_rewind; tburn
+    (* TyAbs *)
+    | [ |- context [ TyAbs _ ]         ]
+      => econstructor; rewrite <- delete_tenv_lift; eapply IHt; tburn;
+         rewrite delete_tenv_lift; tburn 
+   end.
 Qed.
 
-Lemma tm_substition_preserves_typing 
-  :  forall (G:env)(s t:term)(U T:typ)
-  ,  delete ((term,U) :: G) 0 ||- s \: U 
-  -> ((term,U) :: G) ||- t \: T 
-  -> delete ((term,U) :: G) 0 ||- [0 ~> s] t \: T.
+Lemma term_substition_preserves_typing 
+  :  forall (D:kenv)(G:tenv)(s t:term)(U T:typ)
+  ,  D, delete (U :: G) 0 ||- s \: U 
+  -> D, (U :: G) ||- t \: T 
+  -> D, delete (U :: G) 0 ||- [0 ~> s] t \: T.
 Proof.
-  rip; eapply tm_substition_preserves_typing'; tburn. 
+  rip; eapply term_substition_preserves_typing'; tburn. 
+Qed.
+Hint Resolve term_substition_preserves_typing.
+
+Theorem type_preservation
+  :  forall (t t':term)(T:typ)
+  ,  nil, nil ||- t \: T
+  -> t ==> t'
+  -> nil, nil ||- t' \: T.
+Proof.
+  rip; gen t' T; induction t; introh Heval Htyp;
+  inverts Heval; inverts Htyp.
+
+  burn.
+  burn.
+  burn.
+  burn.
+  burn.
+
+  inverts H4.
+  eapply term_substition_preserves_typing. simpl. eassumption. assumption.
+  burn.
+
+  inverts H3.
+  eapply (type_substition_preserves_typing _ nil); burn.
 Qed.
 
+Lemma nat_canonical 
+  :  forall (t : term)
+  ,  value t 
+  -> nil, nil ||- t \: TNat
+  -> (exists n, t = (NConst n)).
+Proof.
+  rip; induction_type t; clean 2.
+Qed.
+Hint Resolve nat_canonical.
 
+Lemma arrow_canonical 
+  :  forall (T1 T2:typ)(t : term)
+  ,  value t 
+  -> nil, nil ||- t \: (TArrow T1 T2)
+  -> (exists t0, t = (Abs T1 t0)).
+Proof.
+  rip; induction_type t; clean 2.
+Qed.
+Hint Resolve arrow_canonical.
 
+Lemma all_canonical 
+  :  forall (T:typ)(t:term)
+  ,  value t 
+  -> nil, nil ||- t \: (TAll T)
+  -> (exists t0, t = (TyAbs t0)).
+Proof.
+  rip; induction_type t; clean 2.
+Qed.
+Hint Resolve all_canonical.
 
+Theorem type_progress
+  :  forall (t t':term)(T:typ)
+  ,  nil, nil ||- t \: T
+  -> (exists t', t ==> t')
+  \/ value t.
+Proof.
+  rip; gen t' T; induction_type t.
+
+  (* Add *)  
+  specialize (IHt1 _ H4).
+  specialize (IHt2 _ H6).
+  inverts IHt1; inverts IHt2.
+  left~; burn.
+  left~; burn.
+  left~. extend (nat_canonical t1); spec. elim Hextend. rip. subst. burn.
+  left~.
+   extend (nat_canonical t1); spec; extend (nat_canonical t2); spec. 
+   inverts Hextend; inverts Hextend0; burn.
+
+   (* App *)
+   specialize (IHt1 _ H4).
+   specialize (IHt2 _ H6).
+   inverts IHt1; inverts IHt2; tburn.
+   extend (arrow_canonical T1 T); spec.
+   specialize (Hextend t1 H H4). inverts Hextend.
+   burn.
+   extend (arrow_canonical T1 T); spec.
+   specialize (Hextend t1 H H4). inverts Hextend.
+   burn.
+
+   (* TyApp *)
+   specialize (IHt _ H4). inverts IHt; tburn.
+   extend (all_canonical T0 t H H4). inverts Hextend.
+   burn.
+Qed.
