src/Repr/Tactics.v
@@ -1,0 +1,5 @@
+
+Require Export Repr.Tactics.All.
+Require Export Repr.Tactics.Rewrite.
+Require Export Repr.Tactics.Burn.
+Require Export Repr.Tactics.Norm.
